src/Examples/StatDb/Refinement.v
@@ -2,6 +2,7 @@ From iris.algebra Require Import auth gmap.
 Require Export CSL.Refinement.
 Require Import StatDb.Impl StatDb.WeakestPre.
 Set Default Proof Using "Type".
+Unset Implicit Arguments.
 
 
 
@@ -17,8 +18,8 @@ Section refinement_triples.
   Definition DBInv := (source_ctx ρ ∗ ∃ N γ, is_lock N γ DBLockInv)%I.
 
   (* TODO: write smart tactics for applying the wp_primitives *)
-  Lemma add_refinement {T} j (K: unit → proc DB.Op T) n:
-    {{{ j ⤇ Bind (Call (DB.Add n)) K ∗ DBInv }}} add n {{{ RET tt; j ⤇ Bind (Ret tt) K }}}.
+  Lemma add_refinement {T} j K `{LanguageCtx DB.Op unit T DB.l K} n:
+    {{{ j ⤇ K (Call (DB.Add n)) ∗ DBInv }}} add n {{{ v, RET v; j ⤇ K (Ret v) }}}.
   Proof.
     iIntros (Φ) "(Hj&#Hsource_inv&Hinv) HΦ".
     iDestruct "Hinv" as (N γ) "#Hinv".
@@ -29,7 +30,7 @@ Section refinement_triples.
     wp_bind. iApply (wp_write with "[$]"). iIntros "!> Hsum".
     wp_bind. iApply (wp_read with "Hcount"). iIntros "!> Hcount".
     wp_bind. iApply (wp_write with "[$]"). iIntros "!> Hcount".
-    iMod (ghost_step_lifting_bind with "Hj Hsource_inv Hsource") as "(Hj&Hsource&_)".
+    iMod (ghost_step_lifting with "Hj Hsource_inv Hsource") as "(Hj&Hsource&_)".
     { do 2 eexists; split; last by eauto. econstructor. }
     { set_solver+. }
     iAssert DBLockInv with "[-HΦ Hlocked Hj]" as "HDB".
@@ -39,8 +40,8 @@ Section refinement_triples.
     iIntros "!> _". by iApply "HΦ".
   Qed.
 
-  Lemma avg_refinement {T} j (K: nat → proc DB.Op T):
-    {{{ j ⤇ Bind (Call (DB.Avg)) K ∗ DBInv }}} avg {{{ n, RET n; j ⤇ Bind (Ret n) K }}}.
+  Lemma avg_refinement {T} j K `{LanguageCtx DB.Op nat T DB.l K}:
+    {{{ j ⤇ K (Call (DB.Avg)) ∗ DBInv }}} avg {{{ n, RET n; j ⤇ K (Ret n) }}}.
   Proof.
     iIntros (Φ) "(Hj&#Hsource_inv&Hinv) HΦ".
     iDestruct "Hinv" as (N γ) "#Hinv".
@@ -49,7 +50,7 @@ Section refinement_triples.
     iDestruct "HDB" as (l) "(Hsource&Hsum&Hcount)".
     wp_bind. iApply (wp_read with "Hsum"). iIntros "!> Hsum".
     wp_bind. iApply (wp_read with "Hcount"). iIntros "!> Hcount".
-    iMod (ghost_step_lifting_bind with "Hj Hsource_inv Hsource") as "(Hj&Hsource&_)".
+    iMod (ghost_step_lifting with "Hj Hsource_inv Hsource") as "(Hj&Hsource&_)".
     { do 2 eexists; split; last by eauto. econstructor. }
     { set_solver+. }
     iAssert DBLockInv with "[-HΦ Hlocked Hj]" as "HDB".
@@ -59,4 +60,67 @@ Section refinement_triples.
     iIntros "!> _".
     wp_ret. by iApply "HΦ".
   Qed.
+
+  (* TODO: stop 'compile' from getting unfolded by the various Iris tactics. *)
+
+  (* TODO: this induction argument is completely generic; so should be bundled
+     for arbitrary layers.  The important points are to show triples for each
+     prim op compilation with some common invariant (here, DBInv) which must
+     be Persistent and must imply source_ctx for some ρ. *)
+  Lemma induction_refinement {T1 T2} j K `{LanguageCtx DB.Op T1 T2 DB.l K} (e: proc DB.Op T1):
+    j ⤇ K e ∗ DBInv ⊢ WP StatDb.Impl.impl.(compile) e {{ v, j ⤇ K (Ret v) }}.
+  Proof.
+    iIntros "(Hj&#Hinv)".
+    iInduction e as [] "IH" forall (j T2 K H0).
+    - destruct op.
+      * iApply (add_refinement j K with "[$]"); eauto.
+      * iApply (avg_refinement j K with "[$]"); eauto.
+    - wp_ret. eauto.
+    - wp_bind.
+      iApply wp_wand_l. iSplitL ""; last first.
+      * iApply ("IH1" $! _ _ (fun x => K (Bind x p2)) with "[] Hj"); try iFrame.
+        { iPureIntro. apply comp_ctx; auto. apply _. }
+      * iIntros (?) "Hj".
+        iMod (ghost_step_bind_ret with "Hj []") as "Hj".
+        { set_solver+. }
+        { iDestruct "Hinv" as "($&?)". }
+        iApply "IH"; auto.
+    - iLöb as "IHloop" forall (init).
+      iMod (ghost_step_loop with "Hj []") as "Hj".
+      { set_solver+. }
+      { iDestruct "Hinv" as "($&?)". }
+      wp_loop.
+      iApply wp_wand_l.
+      iSplitL ""; last first.
+      * rewrite /loop1. simpl.
+        iApply ("IH" $! _ _ _ (fun x => K (Bind x
+                               (fun out => match out with
+                               | ContinueOutcome x => Loop body x
+                               | DoneWithOutcome r => Ret r
+                               end))) with "[] Hj")%proc.
+        { iPureIntro. apply comp_ctx; auto. apply _. }
+      * iIntros (out) "Hj".
+        destruct out.
+        ** iNext.
+           iMod (ghost_step_bind_ret with "Hj []") as "Hj".
+           { set_solver+. }
+           { iDestruct "Hinv" as "($&?)". }
+             by iApply "IHloop".
+        ** iNext.
+           iMod (ghost_step_bind_ret with "Hj []") as "Hj".
+           { set_solver+. }
+           { iDestruct "Hinv" as "($&?)". }
+           by wp_ret.
+   - iMod (ghost_step_spawn with "Hj []") as "(Hj&Hj')".
+     { set_solver+. }
+     { iDestruct "Hinv" as "($&?)". }
+     iDestruct "Hj'" as (j') "Hj'".
+     iApply (wp_spawn with "[Hj'] [Hj]").
+     { iNext. iApply wp_wand_l; iSplitL ""; last first.
+       { iApply ("IH" $! _ _ (fun x => x)); first (iPureIntro; apply _).
+         iFrame. }
+       eauto. }
+     eauto.
+  Qed.
+
 End refinement_triples.
